wip; basic properties of star, sel, upd etc.

pulse/examples/steel_wip/Memory.fst
@@ -1,19 +1,21 @@
 module Memory
 open FStar.Real
-let frac = r:FStar.Real.real{FStar.Real.(0.0R <. r && r <=. 1.0R)}
+module F = FStar.FunctionalExtensionality
+open FStar.FunctionalExtensionality
+let perm = r:FStar.Real.real{FStar.Real.(0.0R <. r && r <=. 1.0R)}
 
 // In the future, we may have other cases of cells
 // for arrays and structs
 noeq
 type cell =
   | Ref : a:Type ->
+          perm:perm ->
           v:a ->
-          perm:frac ->
           cell
 
 let addr = nat
 
-let mem : Type u#(a + 1) = addr -> option (cell u#a)
+let mem : Type u#(a + 1) = addr ^-> option (cell u#a)
 
 let contains_addr (m:mem) (a:addr)
   : bool
@@ -25,29 +27,40 @@ let select_addr (m:mem) (a:addr{contains_addr m a})
 
 let update_addr (m:mem) (a:addr) (c:cell)
   : mem
-  = fun a' -> if a = a' then Some c else m a
+  = F.on _ (fun a' -> if a = a' then Some c else m a')
+
+module T = FStar.Tactics
+
+
+let disjoint_addr (m0 m1:mem) (a:addr)
+  : prop
+  = match m0 a, m1 a with
+    | Some (Ref t0 p0 v0), Some (Ref t1 p1 v1) ->
+      p0 +. p1 <=. 1.0R /\
+      t0 == t1 /\
+      v0 == v1
+
+    | Some _, None
+    | None, Some _
+    | None, None ->
+      True
+
+    | _ ->
+      False
 
 let disjoint (m0 m1:mem)
   : prop
-  = forall a. match m0 a, m1 a with
-         | Some (Ref t0 v0 p0), Some (Ref t1 v1 p1) ->
-           p0 +. p1 <. 1.0R /\
-           t0 == t1 /\
-           v0 == v1
-
-         | Some _, None
-         | None, Some _ ->
-           True
-
-         | _ ->
-           False
+  = forall a. disjoint_addr m0 m1 a
 
 let join (m0:mem) (m1:mem{disjoint m0 m1})
   : mem
-  = fun a ->
-      if contains_addr m0 a
-      then m0 a
-      else m1 a
+  = F.on _ (fun a ->
+      match m0 a, m1 a with
+      | None, None -> None
+      | None, Some x -> Some x
+      | Some x, None -> Some x
+      | Some (Ref a0 p0 v0), Some (Ref a1 p1 v1) ->
+        Some (Ref a0 (p0 +. p1) v0))
 
 ////////////////////////////////////////////////////////////////////////////////
 
@@ -57,7 +70,7 @@ module W = FStar.WellFounded
 
 noeq
 type hprop =
-  | Pts_to : #a:_ -> r:ref a -> perm:frac -> v:a -> hprop
+  | Pts_to : #a:_ -> r:ref a -> perm:perm -> v:a -> hprop
   | And  : hprop -> hprop -> hprop
   | Or   : hprop -> hprop -> hprop
   | Star : hprop -> hprop -> hprop
@@ -70,7 +83,7 @@ let rec interp (p:hprop) (m:mem)
   = match p with
     | Pts_to #a r perm v ->
       m `contains_addr` r /\
-      (let Ref a' v' perm' = select_addr m r in
+      (let Ref a' perm' v' = select_addr m r in
        a == a' /\
        v == v' /\
        perm <=. perm')
@@ -102,11 +115,12 @@ let rec interp (p:hprop) (m:mem)
     | All f ->
       forall x. (W.axiom1 f x; interp (f x) m)
 
-let equiv (p1 p2:hprop) = forall m. interp p1 m <==> interp p2 m
+let equiv (p1 p2:hprop) =
+  forall m. interp p1 m <==> interp p2 m
 
 let hmem (p:hprop) = m:mem{interp p m}
 
-let ptr_perm #a (r:ref a) (p:frac) =
+let ptr_perm #a (r:ref a) (p:perm) =
     Ex (fun v -> Pts_to r p v)
 
 let ptr #a (r:ref a) =
@@ -114,67 +128,126 @@ let ptr #a (r:ref a) =
 
 let sel #a (r:ref a) (m:hmem (ptr r))
   : a
-  = let Ref _ v _ = select_addr m r in
+  = let Ref _ _ v = select_addr m r in
     v
 
-let sel_lemma #a (r:ref a) (p:frac) (m:hmem (ptr_perm r p))
+let sel_lemma #a (r:ref a) (p:perm) (m:hmem (ptr_perm r p))
   : Lemma (let v = sel r m in
            interp (Pts_to r p v) m)
   = ()
 
-let upd #a (r:ref a) (v:a) (m:hmem (ptr r))
-  : mem
-  = let Ref _ _ p = select_addr m r in
-    update_addr m r (Ref a v p)
+let split_mem_ghost (p1 p2:hprop) (m:hmem (p1 `Star` p2))
+  : GTot (ms:(hmem p1 & hmem p2){
+            let m1, m2 = ms in
+            disjoint m1 m2 /\
+            m == join m1 m2})
+  = let open FStar.IndefiniteDescription in
+    let (| m1, p |)
+      : (m1:mem &
+        (exists (m2:mem).
+          m1 `disjoint` m2 /\
+          m == join m1 m2 /\
+          interp p1 m1 /\
+          interp p2 m2))
+        =
+      indefinite_description
+        mem
+        (fun (m1:mem) ->
+          exists (m2:mem).
+            m1 `disjoint` m2 /\
+            m == join m1 m2 /\
+            interp p1 m1 /\
+            interp p2 m2)
+    in
+    let p :
+      (exists (m2:mem).
+        m1 `disjoint` m2 /\
+        m == join m1 m2 /\
+        interp p1 m1 /\
+        interp p2 m2) = p
+    in
+    let _ = FStar.Squash.return_squash p in
+    let (| m2, _ |) =
+      indefinite_description
+        mem
+        (fun (m2:mem) ->
+           m1 `disjoint` m2 /\
+           m == join m1 m2 /\
+           interp p1 m1 /\
+           interp p2 m2)
+    in
+    (m1, m2)
 
-(* Alternatively:
+assume
+private
+val axiom_ghost_to_tot (#a:Type) (#b:a -> Type) ($f: (x:a -> GTot (b x))) (x:a)
+  : Tot (b x)
 
-let upd' #a (r:ref a) (v:a)
-            (frame:hprop) (m:hmem (ptr_perm r 1.0R  `Star` frame))
-  : m:hmem (Pts_to r 1.0R v `Star` frame)
-  = let m0, m1 = FStar.IndefiniteDescription.indefinitedescription ... in
-    join (upd m0 ...) m1
+let split_mem (p1 p2:hprop) (m:hmem (p1 `Star` p2))
+  : Tot (ms:(hmem p1 & hmem p2){
+            let m1, m2 = ms in
+            disjoint m1 m2 /\
+            m == join m1 m2})
+  = axiom_ghost_to_tot (split_mem_ghost p1 p2) m
 
-*)
+let upd #a (r:ref a) (v:a)
+           (frame:hprop) (m:hmem (ptr_perm r 1.0R  `Star` frame))
+  : Tot (m:hmem (Pts_to r 1.0R v `Star` frame))
+  = let m0, m1 = split_mem (ptr_perm r 1.0R) frame m in
+    let m0' = update_addr m0 r (Ref a 1.0R v) in
+    join m0' m1
 
-let upd_lemma #a (r:ref a) (v:a) (m:hmem (ptr r))
-  : Lemma (let m' = upd r v m in
-           interp (Ex (fun p -> Pts_to r p v)) m')
+let mem_equiv (m0 m1:mem) =
+  forall a. m0 a == m1 a
+
+let mem_equiv_eq (m0 m1:mem)
+  : Lemma
+    (requires
+      m0 `mem_equiv` m1)
+    (ensures
+      m0 == m1)
+    [SMTPat (m0 `mem_equiv` m1)]
+  = F.extensionality _ _ m0 m1
+
+let join_commutative (m0 m1:mem)
+  : Lemma
+    (requires
+      disjoint m0 m1)
+    (ensures
+      join m0 m1 `mem_equiv` join m1 m0)
+    [SMTPat (join m0 m1)]
   = ()
 
-let upd_star #a0 (r0:ref a0) (p0:frac) (v0:a0)
-             #a1 (r1:ref a1) (p1:frac{p0 +. p1 >. 1.0R}) (v1:a1)
-             (m:hmem (Pts_to r0 p0 v0 `Star` Pts_to r1 p1 v1))
-  : Lemma (let m' = upd r0 v0 m in
-           interp (Ex (fun p -> Pts_to r0 p v0) `Star` Pts_to r1 p1 v1) m')
-  = let m' = upd r0 v0 m in
-    assert (interp (Ex (fun p -> Pts_to r0 p v0)) m');
-    let aux (m0 m1:mem)
-       : Lemma
-         (requires
-           p0 +. p1 >. 1.0R /\
-           interp (Pts_to r0 p0 v0) m0 /\
-           interp (Pts_to r1 p1 v1) m1 /\
-           disjoint m0 m1 /\
-           m == join m0 m1)
-         (ensures interp (Ex (fun p -> Pts_to r0 p v0) `Star` Pts_to r1 p1 v1) m')
-         [SMTPat (interp (Pts_to r0 p0 v0) m0);
-          SMTPat (interp (Pts_to r1 p1 v1) m1)]
-       = assert (interp (Ex (fun p -> Pts_to r0 p v0)) m');
-         assert (r0 <> r1);
-         assume (interp (Pts_to r1 p1 v1) m);
-         assert (sel r1 m == v1);
-         let Ref _ _ p = select_addr m r0 in
-         assert (m' == update_addr m r0 (Ref a0 v0 p));
-         assume ((update_addr m r0 (Ref a0 v0 p)) r1 == m r1);
-         assert (sel r1 m' == v1);
-         assert (exists p1'. p1' >=. p1 /\ select_addr m' r1 == Ref a1 v1 p1');
-         assert (interp (Pts_to r1 p1 v1) m');
-         assert (interp (Pts_to r0 p0 v0) m');
-         assume (interp (Pts_to r0 p0 v0 `Star` Pts_to r1 p1 v1) m')
-    in
-    assert (exists m0 m1.
-              disjoint m0 m1 /\
-              m == join m0 m1 /\
-              interp (Pts_to r0 p0 v0) m0 /\
-              interp (Pts_to r1 p1 v1) m1)
+let join_associative (m0 m1 m2:mem)
+  : Lemma
+    (requires
+      disjoint m1 m2 /\
+      disjoint m0 (join m1 m2))
+    (ensures
+      disjoint m0 m1 /\
+      disjoint (join m0 m1) m2  /\
+      join m0 (join m1 m2) `mem_equiv` join (join m0 m1) m2)
+    [SMTPat (join m0 (join m1 m2))]
+  = ()
+
+let join_associative2 (m0 m1 m2:mem)
+  : Lemma
+    (requires
+      disjoint m0 m1 /\
+      disjoint (join m0 m1) m2)
+    (ensures
+      disjoint m1 m2 /\
+      disjoint m0 (join m1 m2) /\
+      join m0 (join m1 m2) `mem_equiv` join (join m0 m1) m2)
+    [SMTPat (join (join m0 m1) m2)]
+  = ()
+
+let star_commutative (p1 p2:hprop)
+  : Lemma ((p1 `Star` p2) `equiv` (p2 `Star` p1))
+  = ()
+
+#push-options "--query_stats --z3rlimit_factor 4 --max_fuel 2 --initial_fuel 2 --max_ifuel 2 --initial_ifuel 2"
+let star_associative (p1 p2 p3:hprop)
+  : Lemma ((p1 `Star` (p2 `Star` p3)) `equiv` ((p1 `Star` p2) `Star` p3))
+  = ()
+#pop-options
